src/3d/GenMakefile.fst
@@ -1,6 +1,12 @@
 module GenMakefile
+module OS = OS
+
+type rule_type =
+  | EverParse
+  | CC
 
 type rule_t = {
+  ty: rule_type;
   from: list string;
   to: list string;
   args: string;
@@ -18,7 +24,12 @@ let print_gnu_make_rule
   | [] -> ""
   | a :: q ->
     let rule = Printf.sprintf "%s : %s\n" a (String.concat " " r.from) in
-    let rule = Printf.sprintf "%s\t$(EVERPARSE_CMD) --odir %s %s\n\n" rule output_dir r.args in
+    let cmd =
+      match r.ty with
+      | EverParse -> Printf.sprintf "$(EVERPARSE_CMD) --odir %s" output_dir
+      | CC -> Printf.sprintf "$(CC) -I %s -c" ("$(EVERPARSE_HOME)" `OS.concat` "src" `OS.concat` "3d")
+    in
+    let rule = Printf.sprintf "%s\t%s %s\n\n" rule cmd r.args in
     let rule = List.Tot.fold_left (fun rule ne -> Printf.sprintf "%s%s: %s\n\ttest -f $@ && touch $@\n\n" rule ne a) rule q in
     rule
 
@@ -34,6 +45,7 @@ let produce_types_checked_rule
 : Tot rule_t
 = let types_fst = mk_filename modul "Types.fst" in 
   {
+    ty = EverParse;
     from = types_fst :: List.Tot.map (fun m -> mk_filename m "fsti.checked") (Deps.dependencies g modul);
     to = [mk_filename modul "Types.fst.checked"];
     args = Printf.sprintf "--__micro_step verify %s" types_fst;
@@ -45,6 +57,7 @@ let produce_fsti_checked_rule
 : Tot rule_t
 = let fsti = mk_filename modul "fsti" in
   {
+    ty = EverParse;
     from = fsti :: mk_filename modul "Types.fst.checked" :: List.Tot.map (fun m -> mk_filename m "fsti.checked") (Deps.dependencies g modul);
     to = [mk_filename modul "fsti.checked"];
     args = Printf.sprintf "--__micro_step verify %s" fsti;
@@ -56,6 +69,7 @@ let produce_fst_checked_rule
 : Tot rule_t
 = let fst = mk_filename modul "fst" in
   {
+    ty = EverParse;
     from = fst :: mk_filename modul "fsti.checked" :: List.Tot.map (fun m -> mk_filename m "fsti.checked") (Deps.dependencies g modul);
     to = [mk_filename modul "fst.checked"];
     args = Printf.sprintf "--__micro_step verify %s" fst;
@@ -67,6 +81,7 @@ let produce_types_krml_rule
 : Tot rule_t
 =
   {
+    ty = EverParse;
     from = mk_filename modul "Types.fst.checked" :: List.Tot.map (fun m -> mk_filename m "fst.checked") (Deps.dependencies g modul);
     to = [mk_filename (Printf.sprintf "%s_Types" modul) "krml"];
     args = Printf.sprintf "--__micro_step extract %s" (mk_filename modul "Types.fst");
@@ -78,6 +93,7 @@ let produce_krml_rule
 : Tot rule_t
 =
   {
+    ty = EverParse;
     from = mk_filename modul "fst.checked" :: List.Tot.map (fun m -> mk_filename m "fst.checked") (Deps.dependencies g modul);
     to = [mk_filename modul "krml"];
     args = Printf.sprintf "--__micro_step extract %s" (mk_filename modul "fst");
@@ -88,44 +104,82 @@ let produce_fst_rule
 : FStar.All.ML rule_t
 =
   {
+    ty = EverParse;
     from = all_files;
     to =
       begin
         let types = List.map (fun f -> mk_filename (Options.get_module_name f) "Types.fst") all_files in
         let fsti = List.map (fun f -> mk_filename (Options.get_module_name f) "fsti") all_files in
         let fst = List.map (fun f -> mk_filename (Options.get_module_name f) "fst") all_files in
-        types `List.Tot.append` fsti `List.Tot.append` fst
+        let wrapper_h = List.map (fun f -> mk_filename (Printf.sprintf "%sWrapper" (Options.get_module_name f)) "h") all_files in
+        let wrapper_c = List.map (fun f -> mk_filename (Printf.sprintf "%sWrapper" (Options.get_module_name f)) "c") all_files in
+        types `List.Tot.append` fsti `List.Tot.append` fst `List.Tot.append` wrapper_h `List.Tot.append` wrapper_c
       end;
     args = Printf.sprintf "--__skip_deps --no_batch %s" (String.concat " " all_files);
   }
 
 let produce_h_rule
-  (all_files: list string)
+  (g: Deps.dep_graph)
+  (file: string)
 : FStar.All.ML rule_t
 =
+  let all_files = Deps.collect_and_sort_dependencies_from_graph g [file] in
   {
+    ty = EverParse;
     from =
       List.map (fun f -> mk_filename (Options.get_module_name f) "krml") all_files `List.Tot.append`
       List.map (fun f -> mk_filename (Printf.sprintf "%s_Types" (Options.get_module_name f)) "krml") all_files
       ;
-    to = List.map (fun f -> mk_filename (Options.get_module_name f) "h") all_files;
-    args = Printf.sprintf "--__skip_deps --__produce_c_from_existing_krml %s" (String.concat " " all_files);
+    to = [mk_filename (Options.get_module_name file) "h"; mk_filename (Options.get_module_name file) "c"];
+    args = Printf.sprintf "--__produce_c_from_existing_krml %s" file;
+  }
+
+let produce_o_rule
+  (modul: string)
+: Tot rule_t
+=
+  let c = mk_filename modul "c" in
+  {
+    ty = CC;
+    from = [c; mk_filename modul "h"];
+    to = [mk_filename modul "o"];
+    args = c;
+  }
+
+let produce_wrapper_o_rule
+  (modul: string)
+: Tot rule_t
+=
+  let wc = mk_filename (Printf.sprintf "%sWrapper" modul) "c" in
+  let wh = mk_filename (Printf.sprintf "%sWrapper" modul) "h" in
+  let wo = mk_filename (Printf.sprintf "%sWrapper" modul) "o" in
+  let h = mk_filename modul "h" in
+  {
+    ty = CC;
+    from = [wc; wh; h];
+    to = [wo];
+    args = wc;
   }
 
 let produce_makefile
   (files: list string)
-: FStar.All.ML (list rule_t)
+: FStar.All.ML (list rule_t & list string)
 =
   let g = Deps.build_dep_graph_from_list files in
   let all_files = Deps.collect_and_sort_dependencies_from_graph g files in
   let all_modules = List.map Options.get_module_name all_files in
-  produce_h_rule all_files ::
-  produce_fst_rule all_files ::
-  List.Tot.map (produce_types_checked_rule g) all_modules `List.Tot.append`
-  List.Tot.map (produce_fsti_checked_rule g) all_modules `List.Tot.append`
-  List.Tot.map (produce_fst_checked_rule g) all_modules `List.Tot.append`
-  List.Tot.map (produce_types_krml_rule g) all_modules `List.Tot.append`
-  List.Tot.map (produce_krml_rule g) all_modules
+  let rules =
+    produce_fst_rule all_files ::
+    List.Tot.map (produce_types_checked_rule g) all_modules `List.Tot.append`
+    List.Tot.map (produce_fsti_checked_rule g) all_modules `List.Tot.append`
+    List.Tot.map (produce_fst_checked_rule g) all_modules `List.Tot.append`
+    List.Tot.map (produce_types_krml_rule g) all_modules `List.Tot.append`
+    List.Tot.map (produce_krml_rule g) all_modules `List.Tot.append`
+    List.map (produce_h_rule g) all_files `List.Tot.append`
+    List.Tot.map produce_o_rule all_modules `List.Tot.append`
+    List.Tot.map produce_wrapper_o_rule all_modules
+  in
+  (rules, all_files)
 
 let write_gnu_makefile
   (files: list string)
@@ -133,5 +187,16 @@ let write_gnu_makefile
 =
   let makefile = Options.get_makefile_name () in
   let file = FStar.IO.open_write_file makefile in
-  FStar.IO.write_string file (String.concat "" (List.Tot.map print_gnu_make_rule (produce_makefile files)));
+  let (rules, all_files) = produce_makefile files in
+  FStar.IO.write_string file (String.concat "" (List.Tot.map print_gnu_make_rule rules));
+  let write_all_ext_files (ext_cap: string) (ext: string) : FStar.All.ML unit =
+    let ln =
+      List.map (fun f -> mk_filename (Options.get_module_name f) ext) all_files `List.Tot.append`
+      List.map (fun f -> mk_filename (Printf.sprintf "%sWrapper" (Options.get_module_name f)) ext) all_files
+    in
+    FStar.IO.write_string file (Printf.sprintf "ALL_%s_FILES=%s\n" ext_cap (String.concat " " ln))
+  in
+  write_all_ext_files "H" "h";
+  write_all_ext_files "C" "c";
+  write_all_ext_files "O" "o";
   FStar.IO.close_write_file file
