src/3d/Batch.fsti
@@ -27,15 +27,14 @@ val check_inplace_hashes
   (files_3d_c: list string)
 : ML unit
 
-val produce_and_postprocess_c
+val produce_and_postprocess_one_c
   (clang_format: bool)
   (clang_format_executable: string)
-  (skip_makefiles: bool)
-  (cleanup: bool)
-  (no_everparse_h: bool)
   (save_hashes: bool)
   (out_dir: string)
-  (files_and_modules: list (string & string))
+  (file: string)
+  (modul: string)
+  (dep_files_and_modules: list (string & string))
 : ML unit
 
 val postprocess_fst
